theories/Sem/Semantics.v
@@ -61,23 +61,21 @@ Axiom offset_ptr_0 : forall b,
  *)
 Parameter genv : Type.
 
-
 Parameter has_type : val -> type -> Prop.
 
-Axiom has_type_pointer : forall v ty, has_type v (Tpointer ty) ->
-                                 exists p, v = Vptr p.
+Axiom has_type_pointer : forall v ty, has_type v (Tpointer ty) -> exists p, v = Vptr p.
 
-Definition bound (bits : nat) (sgn : bool) (v : Z) : Prop :=
+Definition bound (bits : size) (sgn : signed) (v : Z) : Prop :=
   if sgn then
-    (-Z.pow 2 (Z.of_nat bits - 1) < v < Z.pow 2 (Z.of_nat bits - 1) - 1)%Z
+    (-Z.pow 2 (Z.of_N bits - 1) < v < Z.pow 2 (Z.of_N bits - 1) - 1)%Z
   else
-    (0 <= v < Z.pow 2 (Z.of_nat bits))%Z.
+    (0 <= v < Z.pow 2 (Z.of_N bits))%Z.
 
-Axiom has_int_type : forall (sz : nat) (sgn : bool) z,
-    bound sz sgn z <-> has_type (Vint z) (Tint (Some sz) sgn).
+Axiom has_int_type : forall sz (sgn : signed) z,
+    bound sz sgn z <-> has_type (Vint z) (Tint sz sgn).
 
-Axiom has_char_type : forall (sgn : bool) z,
-    bound 8 sgn z <-> has_type (Vint z) (Tchar (Some 8) sgn).
+Axiom has_char_type : forall sz (sgn : signed) z,
+    bound sz sgn z <-> has_type (Vint z) (Tchar sz sgn).
 
 Axiom has_type_qual : forall t q x,
     has_type x (drop_qualifiers t) ->
@@ -87,8 +85,6 @@ Hint Resolve has_type_qual : has_type.
 
 
 
-(* alignment of a type *)
-Parameter align_of : forall {c : genv} (t : type) (e : N), Prop.
 
 (* address of a global variable *)
 Parameter glob_addr : genv -> obj_name -> ptr -> Prop.
@@ -97,14 +93,22 @@ Parameter glob_addr : genv -> obj_name -> ptr -> Prop.
 Parameter offset_of : forall (resolve : genv) (t : type) (f : ident) (e : Z), Prop.
 Parameter parent_offset : forall (resolve : genv) (t : globname) (f : globname) (e : Z), Prop.
 
+Parameter pointer_size : N. (* in bytes *)
+
+
+(* sizeof() *)
 Parameter size_of : forall (resolve : genv) (t : type) (e : N), Prop.
+Axiom size_of_unique : forall {c : genv} t sz sz',
+    @size_of c t sz ->
+    @size_of c t sz' ->
+    sz = sz'.
+
 Axiom size_of_int : forall {c : genv} s w,
-    @size_of c (Tint (Some w) s) (N.div (N.of_nat w) 8).
+    @size_of c (Tint w s) (N.div (w + 7) 8).
 Axiom size_of_char : forall {c : genv} s w,
-    @size_of c (Tchar (Some w) s) (N.div (N.of_nat w) 8).
+    @size_of c (Tchar w s) (N.div (w + 7) 8).
 Axiom size_of_bool : forall {c : genv},
     @size_of c Tbool 1.
-Parameter pointer_size : N. (* in bytes *)
 Axiom size_of_pointer : forall {c : genv} t,
     @size_of c (Tpointer t) pointer_size.
 Axiom size_of_qualified : forall {c : genv} t sz q,
@@ -112,11 +116,12 @@ Axiom size_of_qualified : forall {c : genv} t sz q,
     @size_of c (Tqualified q t) sz.
 Axiom size_of_array : forall {c : genv} t n sz,
     @size_of c t sz ->
-    @size_of c (Tarray t n) (sz * N.of_nat n).
-Axiom size_of_unique : forall {c : genv} t sz sz',
-    @size_of c t sz ->
-    @size_of c t sz' ->
-    sz = sz'.
+    @size_of c (Tarray t n) (sz * n).
+
+(* alignof() *)
+Parameter align_of : forall {resolve : genv} (t : type) (e : N), Prop.
+
+
 
 (* operator semantics *)
 Parameter eval_unop : forall {resolve : genv}, UnOp -> forall (argT resT : type) (arg res : val), Prop.
@@ -146,24 +151,24 @@ Definition eval_int_ptr_op (bo : BinOp) (o : Z -> Z -> Z) : Prop :=
 Axiom eval_int_ptr_add :
   ltac:(let x := eval hnf in (eval_int_ptr_op Badd Z.add) in refine x).
 
-Axiom eval_ptr_ptr_add :
+Axiom eval_ptr_ptr_sub :
   forall resolve t w p o1 o2 p' base sz,
     size_of resolve t sz ->
     p = offset_ptr base (Z.of_N sz * o1) ->
     p' = offset_ptr base (Z.of_N sz * o2) ->
     eval_binop (resolve:=resolve) Bsub
-               (Tpointer t) (Tpointer t) (Tint w true)
+               (Tpointer t) (Tpointer t) (Tint w Signed)
                p            p'           (Vint (o1 - o2)).
 
 Definition eval_int_op (bo : BinOp) (o : Z -> Z -> Z) : Prop :=
-  forall resolve w (s : bool) (a b c : Z) bytes,
+  forall resolve w s (a b c : Z) bytes,
     size_of resolve (Tint w s) bytes ->
     c = (if s then o a b else Z.modulo (o a b) (Z.pow 2 (8 * Z.of_N bytes))) ->
     has_type (Vint c) (Tint w s) ->
     eval_binop (resolve:=resolve) bo (Tint w s) (Tint w s) (Tint w s) (Vint a) (Vint b) (Vint c).
 
 Definition eval_int_bin_op (bo : BinOp) (o : Z -> Z -> Z) : Prop :=
-  forall resolve w (s : bool) (a b c : Z) bytes,
+  forall resolve w s (a b c : Z) bytes,
     size_of resolve (Tint w s) bytes ->
     c = (if s then o a b else Z.modulo (o a b) (Z.pow 2 (8 * Z.of_N bytes))) ->
     eval_binop (resolve:=resolve) bo (Tint w s) (Tint w s) (Tint w s) (Vint a) (Vint b) (Vint c).
@@ -182,13 +187,13 @@ Axiom eval_and :
 Axiom eval_xor :
   ltac:(let x := eval hnf in (eval_int_op Bxor Z.lxor) in refine x).
 Axiom eval_div :
-  forall resolve (w : option nat) (s : bool) (a b c : Z),
+  forall resolve (w : size) (s : signed) (a b c : Z),
     b <> 0%Z ->
     c = Z.quot a b ->
     has_type (Vint c) (Tint w s) ->
     eval_binop (resolve:=resolve) Bdiv (Tint w s) (Tint w s) (Tint w s) (Vint a) (Vint b) (Vint c).
 Axiom eval_mod :
-  forall resolve (w : option nat) (s : bool) (a b c : Z),
+  forall resolve (w : size) (s : signed) (a b c : Z),
     b <> 0%Z ->
     c = Z.rem a b ->
     has_type (Vint c) (Tint w s) ->
